proof/AdequacySound.v
@@ -12,6 +12,7 @@ Require Import Skeleton ModSem Mod Sem.
 Require Import SimSymb SimMem SimMod SimModSem SimProg (* SimLoad *) SimProg.
 Require Import SemProps Ord.
 Require Import Sound Preservation.
+Require Import Memory.
 
 Set Implicit Arguments.
 
@@ -39,108 +40,168 @@ Section ADQSOUND.
   Let skenv_link_tgt := sk_link_tgt.(Sk.load_skenv).
 
   (* stack can go preservation when su0 is given *)
-  Inductive sound_stack (su0: Sound.t): list Frame.t -> Prop :=
+  Inductive sound_stack (su0: Sound.t) (args: Args.t) (m_arg: mem): list Frame.t -> Prop :=
   | sound_stack_nil
     :
-      sound_stack su0 []
+      sound_stack su0 args m_arg []
   | sound_stack_cons
-      su_tail
-      ms lst0 tail
-      (TL: sound_stack su_tail tail)
-      (HD: forall
+      su_tail m_tail args_tail tail
+      ms lst0
+      (TL: sound_stack su_tail args_tail m_tail tail)
+      (K: forall
           sound_state_all
           (PRSV: local_preservation ms sound_state_all)
         ,
-          (<<SUST: sound_state_all su0 lst0>>)
+          (<<SUST: sound_state_all su0 m_arg lst0>>)
           /\
           (<<K: forall
               retv lst1
-              args
-              (SURETV: Sound.retv su0 retv)
-              (MLE: Sound.mle su0 args.(Args.m) retv.(Retv.m))
+              su_greatest
+              (GR: Sound.get_greatest args su_greatest)
+              (SURETV: Sound.retv su_greatest retv)
+              (MLE: Sound.mle su_greatest args.(Args.m) retv.(Retv.m))
               (AFTER: ms.(ModSem.after_external) lst0 retv lst1)
             ,
-              sound_state_all su_tail lst1>>)
+              sound_state_all su0 m_arg lst1>>)
       )
+      (GR: Sound.get_greatest args_tail su0)
+      (EX: exists sound_state_ex, local_preservation ms sound_state_ex)
       (* sound_state_ex *)
       (* (PRSV: local_preservation ms sound_state_ex) *)
       (* (HD: sound_state_ex su0 lst0) *)
     :
-      sound_stack su0 ((Frame.mk ms lst0) :: tail)
+      sound_stack su0 args m_arg ((Frame.mk ms lst0) :: tail)
   .
 
-  Inductive sound_state (su0: Sound.t): state -> Prop :=
+  Inductive sound_state (su0: Sound.t): mem -> state -> Prop :=
   | sound_state_normal
-      su_tail ms lst0 tail
-      (TL: sound_stack su_tail tail)
+      su_tail args_tail m_tail tail
+      ms lst0
+      m_arg
+      (GR: Sound.get_greatest args_tail su0)
+      (TL: sound_stack su_tail args_tail m_tail tail)
       (HD: forall
           sound_state_all
           (PRSV: local_preservation ms sound_state_all)
         ,
-          <<SUST: sound_state_all su0 lst0>>)
+          <<SUST: sound_state_all su0 m_arg lst0>>)
+      (EX: exists sound_state_ex, local_preservation ms sound_state_ex)
     :
-      sound_state su0 (State ((Frame.mk ms lst0) :: tail))
+      sound_state su0 m_arg (State ((Frame.mk ms lst0) :: tail))
   | sound_state_call
-      su_tail frs
-      (STK: sound_stack su_tail frs)
+      su_tail m_tail frs
       args
+      (GR: Sound.get_greatest args su0)
       (ARGS: Sound.args su0 args)
+      (STK: sound_stack su_tail args m_tail frs)
     :
-      sound_state su0 (Callstate args frs)
+      sound_state su0 m_tail (Callstate args frs)
   .
 
   Lemma sound_init
         st0
         (INIT: sem_src.(Smallstep.initial_state) st0)
     :
-      exists su0, sound_state su0 st0
+      exists m_init su0, sound_state su0 m_init st0
   .
   Proof.
     inv INIT.
-    esplits; eauto. econs; eauto.
-    - econs; eauto.
+    esplits; eauto. econs; s; eauto.
+    - admit "this should hold".
     - eapply Sound.top_args.
+    - econs; eauto.
   Unshelve.
-    all: exact Sound.top.
+    all: try exact Sound.top.
+    all: try exact Mem.empty.
   Qed.
 
   Lemma sound_progress
-        su0 st0 tr st1
-        (SUST: sound_state su0 st0)
+        su0 st0 m_init0 tr st1
+        (SUST: sound_state su0 m_init0 st0)
         (STEP: Step sem_src st0 tr st1)
     :
-      <<SUST: exists su1, sound_state su1 st1>>
+      <<SUST: exists su1 m_init1, sound_state su1 m_init1 st1>>
   .
   Proof.
     inv STEP.
     - (* CALL *)
       inv SUST. ss.
-      assert(exists su_greatest, su_greatest.(Sound.args) args).
-      { admit "". }
-      des.
-      exists su_greatest. econs; eauto. econs; eauto.
+      generalize (Sound.greatest_ex args). i; des.
+      exists su_gr.
+      esplits; eauto.
+      econs; eauto.
+      { eapply Sound.greatest_spec; eauto. }
+      econs; eauto.
       ii.
       dsplits; eauto.
       inv PRSV. exploit CALL; eauto. i; des.
-      assert(su_lifted = su_greatest).
-      { admit "". }
+      ii.
+      assert(su_greatest = su_gr0).
+      { eapply Sound.greatest_dtm; eauto. }
       clarify.
-      ii. inv PRSV.
-      dup PRSV. inv PRSV. dsplits; eauto. i. exploit CALL; eauto. i; des.
+      eapply K; eauto.
     - (* INIT *)
       inv SUST. ss. des_ifs.
-      inv STK.
-      { esplits; eauto. econs; eauto. econs; eauto.
-        - econs; eauto.
-        - ii. inv PRSV. dsplits; eauto.
-          + ii.
-            (* exploit CALL; eauto. *)
-            admit "".
-      }
-      esplits; eauto. econs; eauto. econs; eauto.
-      { econs; eauto. }
-      i. inv PRSV. dsplits; eauto.
-      ii. exploit CALL; eauto.
+
+      esplits; eauto.
+      econs; eauto.
+      + ii. inv PRSV. exploit INIT0; eauto.
+      + inv MSFIND. ss. rr in SIMPROG. rewrite Forall_forall in *.
+        des; clarify.
+        { eapply system_local_preservation. }
+        u in MODSEM.
+        rewrite in_map_iff in MODSEM. des; clarify.
+        exploit SIMPROG.
+        { admit "somehow". }
+        i; des. inv H.
+        admit "somehow".
+      (* inv STK. *)
+      (* { esplits; eauto. econs; eauto. *)
+      (*   - econs; eauto. *)
+      (*   - ii. inv PRSV. dsplits; eauto. *)
+      (*     + ii. *)
+      (*       (* exploit CALL; eauto. *) *)
+      (*       admit "". *)
+      (* } *)
+      (* esplits; eauto. econs; eauto. econs; eauto. *)
+      (* { econs; eauto. } *)
+      (* i. inv PRSV. dsplits; eauto. *)
+      (* ii. exploit CALL; eauto. *)
+    - (* INTERNAL *)
+      inv SUST. ss.
+      esplits; eauto. econs; eauto.
+      i. dup PRSV. inv PRSV. eapply STEP; eauto.
+      + eapply HD; eauto.
+      + split; ii; ModSem.tac.
+    - (* RETURN *)
+      inv SUST. ss. rename ms into ms_top.
+      bar.
+      inv TL. ss.
+      unfold Frame.update_st. s.
+      bar.
+      des. dup EX. inv EX. exploit RET; eauto.
+      { eapply HD; eauto. }
+      bar.
+      i; des.
+      esplits; eauto. econs; try apply TL0; eauto.
+      ii. specialize (K sound_state_all PRSV).
+      eapply K; eauto.
+      rp; eauto.
+  Unshelve.
+  Qed.
+      dup PRSV. inv PRSV.
+      exploit RET; ss; eauto.
+      exploit K; eauto. i; des.
+      eapply K0; eauto.
+      exploit RET; eauto.
+      { eapply HD; eauto. }
+      {
+      inv STK. inv TL.
+      esplits; eauto. econs; eauto. econs; eauto. ss.
+      assert(RETV: Sound.retv su0 retv).
+      { admit "". }
+      i. dup PRSV. inv PRSV.
+    - 
     - (* INTERNAL *)
       inv SUST. inv STK. ss.
       esplits; eauto.
